a couple of updates, mainly in the translation from HSL to CFL

examples/dev/sw/working/0.2/Tree.sml
@@ -1,0 +1,33 @@
+structure Tree  = 
+struct
+  type size = int
+
+datatype stm = SEQ of stm * stm
+             | LABEL of Temp.label
+             | JUMP of Temp.label
+             | CJUMP of exp * Temp.label
+	     | MOVE of exp * exp
+             | EXP of exp
+
+     and exp = BINOP of binop * exp * exp
+	     | RELOP of relop * exp * exp
+             | MEM of exp
+             | TEMP of Temp.temp
+             | ESEQ of stm * exp
+             | NAME of Temp.label
+             | NCONST of Arbint.int
+	     | WCONST of Arbint.int
+	     | CALL of exp * exp
+	     | PAIR of exp * exp
+
+      and binop = PLUS | MINUS | MUL | DIV 
+                | AND | OR | LSHIFT | RSHIFT | ARSHIFT | XOR | ROR
+
+      and relop = EQ | NE | LT | GT | LE | GE 
+	        | CC | LS | HI | CS
+
+  fun pair2list (PAIR(v1, v2)) =
+        (pair2list v1) @ (pair2list v2)
+   |  pair2list v = [v]
+
+end
